theories/Symbolic/UnifLogic.v
@@ -1199,12 +1199,159 @@ Module Type UnifLogicOn
     Qed.
   End ModalRel.
 
+
+  Module RSolve.
+    Import logicalrelation logicalrelation.notations iris.bi.interface notations ModalNotations iris.proofmode.tactics iris.proofmode.environments.
+
+    Class RefineCompat `(R : Rel AT A) (v : A)  w (vs : AT w) (Ob : Pred w) :=
+      MkRefineCompat {
+          refine_compat_lemma : Ob ⊢ ℛ⟦ R ⟧ v vs
+        }.
+    #[export] Hint Mode RefineCompat - - - + + + - : typeclass_instances.
+    #[global] Arguments refine_compat_lemma {AT A R v w vs Ob} rci : rename.
+    #[global] Arguments RefineCompat {AT A} R v w vs Ob%I.
+    #[global] Arguments MkRefineCompat {AT A R v w vs Ob%I} rci : rename.
+
+    Program Definition refine_compat_impl `{RA : Rel AT A} `{RB : Rel BT B} {f v w fs vs} {Pf}
+      (compatf : RefineCompat (RA -> RB) f w fs Pf) : RefineCompat RB (f v) w (fs vs) (Pf ∗ RSat RA v vs) :=
+      MkRefineCompat _.
+    Next Obligation.
+      iIntros (AT A RA BT B RB f v w fs vs Pf compatf) "[Hcf Hv]".
+      now iApply (refine_compat_lemma compatf with "Hcf").
+    Qed.
+
+    (* Outside section because Coq doesn't allow to put it inside (?) *)
+    (* The Hint Resolve used "simple apply", which wasn't instantiating evars sufficiently strongly. Hint Extern with eapply works better. *)
+    #[export] Hint Extern 1 (RefineCompat ?RB (?f ?v) ?w (?fs ?vs) _) => eapply (refine_compat_impl (RB := RB) (fs := fs) (vs := vs) (f := f) (v := v) (w := w)) : typeclass_instances.
+
+    #[export] Program Instance refine_compat_forall {𝑲} {AT : forall K : 𝑲, TYPE} {A : forall K : 𝑲, Type} (RA : forall K, Rel (AT K) (A K)) {f w fs k P}
+      (compatf : RefineCompat (RForall RA) f w fs P) : RefineCompat (RA k) (f k) w (fs k) P :=
+      MkRefineCompat _.
+    Next Obligation.
+      iIntros (𝑲 AT A RA f w fs k P compatf) "Hcf".
+      now iApply (refine_compat_lemma compatf with "Hcf").
+    Qed.
+
+    Ltac rsolve_step :=
+      first [
+          (lazymatch goal with
+           | |- envs_entails _ (ℛ⟦□ᵣ _⟧ _ _) => iIntros (? ?) "!>"
+           | |- envs_entails _ (ℛ⟦_ -> _⟧ _ _) => iIntros (? ?) "#?"
+           end)
+        | lazymatch goal with
+          | |- envs_entails _ (ℛ⟦ ?R ⟧ ?v ?vs) =>
+              (iApply (refine_compat_lemma (R := R) (vs := vs));
+               lazymatch goal with | |- RefineCompat _ _ _ _ _ => fail | _ => idtac end
+              )
+          | |- envs_entails _ (_ ∗ _) => iSplit
+          | |- envs_entails _ (unconditionally _) => iIntros (? ?) "!>"
+          end
+        ].
+
+    Ltac rsolve :=
+      iStartProof;
+      repeat rsolve_step; try done;
+      (* After walking through the symbolic computation using the above lemmas,
+       * we try to apply induction hypotheses.
+       * To do this, we determine the right world to apply the IH in by looking at the current goal.
+       *)
+      repeat match goal with
+        | H : (forall (w : World), _) |- @envs_entails (@bi_pred ?w) _ _ => specialize (H w)
+        | H : (forall (w : World), _) |- @envs_entails _ _ (@logicalrelation.RSat _ _ _ _ ?w _) => specialize (H w)
+        | H : ⊢ ?P |- envs_entails _ ?P => (try iApply H); clear H
+        end.
+
+    Class RefineCompatGen (w : World) (P : Pred w) (Ob : Pred w) (withbase : bool):=
+      MkRefineCompatGen {
+          refine_compat_gen_lemma : Ob ⊢ P
+        }.
+    #[global] Arguments RefineCompatGen [w] P%I Ob%I withbase.
+    #[global] Arguments MkRefineCompatGen {w} {P} _%I _ {_}.
+    #[global] Arguments refine_compat_gen_lemma {w} P%I {Ob} withbase rcg : rename.
+
+    #[export] Program Instance refine_compat_gen_step `(R : Rel AT A) (v : A) (w : World) (vs : AT w) Ob1 Ob2 b
+      (rc : RefineCompat R v w vs Ob1)
+      (iter : RefineCompatGen Ob1 Ob2 b) :
+      RefineCompatGen (ℛ⟦ R ⟧ v vs) Ob2 b := MkRefineCompatGen Ob2 _.
+    Next Obligation.
+      iIntros (AT A R v w vs Ob1 Ob2 b rc iter) "H".
+      iApply (refine_compat_lemma with "[H]").
+      now iApply (refine_compat_gen_lemma with "[H]").
+    Qed.
+
+    #[export] Program Instance refine_compat_gen_base_true {w} {b} :
+      RefineCompatGen (w := w) True emp b := MkRefineCompatGen emp _.
+    Next Obligation.
+      now iIntros.
+    Qed.
+
+    #[export] Program Instance refine_compat_gen_base_emp {w} {b} :
+      RefineCompatGen (w := w) emp emp b := MkRefineCompatGen emp _.
+    Next Obligation.
+      now iIntros.
+    Qed.
+
+    #[export] Program Instance refine_compat_gen_base {w} (P : Pred w):
+      RefineCompatGen (w := w) P P true | 10 := MkRefineCompatGen P _.
+    Next Obligation.
+      now iIntros.
+    Qed.
+
+    Class ObSep {w} (P1 P2 P3 : Pred w) : Prop :=
+      obsep_equiv : P1 ∗ P2 ⊣⊢ P3.
+    #[export] Instance obsep_empL {w} {P : Pred w} : ObSep emp%I P P.
+    Proof. apply bi.emp_sep. Qed.
+    #[export] Instance obsep_empR {w} {P : Pred w} : ObSep P emp%I P.
+    Proof. apply bi.sep_emp. Qed.
+    #[export] Instance obsep_sep {w} {P1 P2 : Pred w} : ObSep P1 P2 (P1 ∗ P2)%I | 1.
+    Proof. done. Qed.
+
+    #[export] Program Instance refine_compat_gen_split {w} {P1 P2 : Pred w} {Ob1 Ob2 Ob} {b}
+      (rcg1 : RefineCompatGen P1 Ob1 b) (rcg2 : RefineCompatGen P2 Ob2 b) {_ : ObSep Ob1 Ob2 Ob} :
+      RefineCompatGen (w := w) (P1 ∗ P2) Ob b | 1 := MkRefineCompatGen Ob _.
+    Next Obligation.
+      iIntros (w P1 P2 Ob1 Ob2 Ob b rcg1 rcg2 obsep) "H".
+      rewrite -(obsep_equiv (ObSep := obsep)).
+      iDestruct "H" as "(H1 & H2)".
+      iSplitL "H1".
+      - iApply (refine_compat_gen_lemma with "H1").
+      - iApply (refine_compat_gen_lemma with "H2").
+    Qed.
+
+    Ltac rsolve2_step :=
+      first [
+          (lazymatch goal with
+           | |- envs_entails _ (ℛ⟦□ᵣ _⟧ _ _) => iIntros (? ?) "!>"
+           | |- envs_entails _ (ℛ⟦_ -> _⟧ _ _) => iIntros (? ?) "#?"
+           end)
+        | lazymatch goal with
+          | |- envs_entails _ ?P => iApply (refine_compat_gen_lemma P true)
+          | |- envs_entails _ (unconditionally _) => iIntros (? ?) "!>"
+          end
+        ].
+
+    Ltac rsolve2 :=
+      iStartProof;
+      progress rsolve2_step; try done;
+      (* After walking through the symbolic computation using the above lemmas,
+       * we try to apply induction hypotheses.
+       * To do this, we determine the right world to apply the IH in by looking at the current goal.
+       *)
+      repeat match goal with
+        | H : (forall (w : World), _) |- @envs_entails (@bi_pred ?w) _ _ => specialize (H w)
+        | H : (forall (w : World), _) |- @envs_entails _ _ (@logicalrelation.RSat _ _ _ _ ?w _) => specialize (H w)
+        | H : ⊢ ?P |- envs_entails _ ?P => (try iApply H); clear H
+        end.
+  End RSolve.
+
+
   Section LRCompat.
     Import notations.
     Import logicalrelation.
     Import logicalrelation.notations.
     (* Import ModalNotations. *)
     Import iris.proofmode.tactics.
+    Import RSolve.
     
     Lemma refine_term_val {w τ v} : ⊢ (ℛ⟦RVal τ⟧ v (term_val τ v) : Pred w).
     Proof. unfold RVal, RInst. crushPredEntails3. Qed.
@@ -1355,9 +1502,18 @@ Module Type UnifLogicOn
       - now rewrite instpred_prop instprop_subst.
     Qed.
 
+    #[export] Instance refine_compat_instprop_subst {Σ} {T : LCtx -> Type} `{InstPredSubst T}
+      {vs : T Σ} {w : World} :
+      RefineCompat ((RInst (Sub Σ) (Valuation Σ) -> RInstPropIff T)) (instprop vs) w (subst vs : Sub Σ w -> T w)%I emp :=
+      MkRefineCompat (refine_instprop_subst _).
+
     Lemma refine_lift {AT A} `{InstLift AT A} {w : World} (a : A) :
       ⊢ ℛ⟦RInst AT A⟧ a (lift a : AT w).
     Proof. iApply lift_repₚ. Qed.
+
+    #[export] Instance refine_compat_lift `{InstLift AT A} {w : World} (a : A) :
+      RefineCompat (RInst AT A) a w (lift a) _ :=
+      MkRefineCompat (refine_lift a).
 
     Import ModalNotations. 
     Section WithNotations.
@@ -1464,6 +1620,21 @@ Module Type UnifLogicOn
       now rewrite instprop_subst inst_subst !inst_sub_cat_left
         inst_pattern_match_term_reverse inst_sub_cat_right eq.
     Qed.
+
+    Lemma refine_pattern_match_val_term_reverse {N} {w : World} {σ}
+      {pat : @Pattern N σ} {ι} :
+      ⊢ ℛ⟦RNEnv N (PatternCaseCtx ι) -> RVal σ⟧ (pattern_match_val_reverse pat ι) (pattern_match_term_reverse pat ι : _ -> STerm σ w).
+    Proof.
+      unfold RSat, RNEnv, RVal, RInst, RImpl, repₚ.
+      intros; crushPredEntails3.
+      rewrite inst_pattern_match_term_reverse.
+      now subst.
+    Qed.
+
+    #[export] Instance refine_compat_pattern_match_val_term_reverse {N} {w : World} {σ}
+      {pat : @Pattern N σ} {ι} :
+        RefineCompat (RNEnv N (PatternCaseCtx ι) -> RVal σ) (pattern_match_val_reverse pat ι) w (pattern_match_term_reverse pat ι) _ :=
+      MkRefineCompat refine_pattern_match_val_term_reverse.
 
     Import ctx.notations.
     Lemma refine_pattern_match_var {w : World} {σ} {v : Val σ} {x : LVar} {xIn : ctx.In (x∷σ) w}
@@ -1600,6 +1771,72 @@ Module Type UnifLogicOn
     Qed.
 
   End LRCompat.
+
+  Import logicalrelation RSolve.
+  Import env.notations.
+  Import ctx.notations.
+  Import ModalNotations.
+  
+  (* Outside the LRCompat section because of Coq restriction *)
+  #[export] Instance refine_compat_term_val {σ} {v w} : RefineCompat (RVal σ) v w (term_val σ v) _ :=
+    MkRefineCompat refine_term_val.
+
+  Definition refine_compat_inst_persist {AT A} `{InstSubst AT A, @SubstLaws AT _} {v} {w1 w2} {ω : Acc w1 w2} {t} :
+    RefineCompat (RInst AT A) v w2 (persist t ω) _ :=
+    MkRefineCompat (refine_inst_persist _).
+  #[global] Opaque refine_compat_inst_persist.
+  #[export] Hint Extern 0 (RefineCompat _ ?v _ (persist ?t ?ω) _) => refine (refine_compat_inst_persist (v := v) (t := t) (ω := ω)) : typeclass_instances.
+
+  #[export] Instance refine_compat_inst_persist_term {σ} {v} {w1 w2} {ω : Acc w1 w2} {t} :
+    RefineCompat (RVal σ) v w2 (persist__term t ω) _ :=
+    MkRefineCompat (refine_inst_persist _).
+
+  Definition refine_compat_term_binop {w τ1 τ2 τ3} {op : BinOp τ1 τ2 τ3} {a1 sa1 a2 sa2} :
+    RefineCompat (RVal τ3) (bop.eval op a1 a2)  w (term_binop op sa1 sa2) _ :=
+    MkRefineCompat refine_term_binop.
+  #[global] Opaque refine_compat_term_binop.
+  #[export] Hint Extern 0 (RefineCompat (RVal _) _ _ (term_binop ?binop _ _) _) => ( refine (refine_compat_term_binop (op := binop)) ) : typeclass_instances.
+
+  #[export] Instance refine_compat_formula_bool {w : World} {v} {sv : Term w ty.bool} :
+    RefineCompat RFormula (v = true) w (formula_bool sv) _ :=
+    MkRefineCompat refine_formula_bool.
+
+  Definition refine_compat_formula_relop {w : World} {σ v1 v2} {sv1 sv2 : Term w σ}  {relop : RelOp σ} :
+    RefineCompat RFormula (bop.eval_relop_prop relop v1 v2) w (formula_relop relop sv1 sv2) _ :=
+    MkRefineCompat refine_formula_relop.
+  #[global] Opaque refine_compat_formula_relop.
+  #[export] Hint Extern 0 (RefineCompat RFormula _ _ (formula_relop ?relop _ _) _) => ( refine (refine_compat_formula_relop (relop := relop)) ) : typeclass_instances.
+
+  #[export] Instance refine_compat_chunk_ptsreg {w σ} {pc a ta} :
+    RefineCompat RChunk (chunk_ptsreg pc a) w(chunk_ptsreg (σ := σ) pc ta) _ :=
+    MkRefineCompat refine_chunk_ptsreg.
+
+  #[export] Instance refine_compat_chunk_user {w c vs svs} :
+    RefineCompat RChunk (chunk_user c vs) w (chunk_user c svs) _ :=
+    MkRefineCompat refine_chunk_user.
+
+  #[export] Instance refine_compat_env_snoc {Δ : Ctx Ty} {τ} {w : World} {vs : Env Val Δ} {svs : Env (Term w) Δ} {v : Val τ} {sv : Term w τ} :
+    RefineCompat (REnv (Δ ▻ τ)) (vs ► ( τ ↦ v ))%env w (svs ► (τ ↦ sv ))%env _ :=
+    MkRefineCompat refine_env_snoc.
+
+  #[export] Instance refine_compat_sub_snoc {τ : Ty} {Γ : LCtx} {x : LVar}
+    {w : World} {vs : NamedEnv Val Γ} {svs : NamedEnv (Term w) Γ}
+    {v : Val τ} {sv : Term w τ} :
+    RefineCompat (RNEnv LVar (Γ ▻ x∷τ)) (vs.[x∷τ ↦ v])%env w (sub_snoc svs (x∷τ) sv) _ :=
+    MkRefineCompat refine_sub_snoc.
+
+  #[export] Instance refine_compat_env_nil {w : World} {vs : Env Val [ctx]} {svs : Env (Term w) [ctx]} :
+    RefineCompat (REnv [ctx]) vs  w svs _ :=
+    MkRefineCompat refine_env_nil.
+
+  #[export] Instance refine_compat_named_env_sub_acc_trans {Σ : LCtx} {w1 w2 : World} {ι : Valuation Σ} {ω1 : wlctx Σ ⊒ w1} {ω2 : w1 ⊒ w2}:
+    RefineCompat (RNEnv LVar (wlctx Σ)) ι w2 (sub_acc (acc_trans ω1 ω2)) _ :=
+    MkRefineCompat refine_namedenv_sub_acc_trans.
+
+  (* #[export] Instance refine_compat_named_env_sub_acc {Σ : LCtx} {w : World} {ι : Valuation Σ} {ω : wlctx Σ ⊒ w} : *)
+  (*   RefineCompat (RNEnv LVar (wlctx Σ)) ι w (sub_acc ω) _ | 10 := *)
+  (*   MkRefineCompat refine_namedenv_sub_acc. *)
+
 
   Import notations logicalrelation.notations logicalrelation iris.proofmode.tactics.
   Global Hint Extern 0 (environments.envs_entails _ (ℛ⟦ RUnit ⟧ _ _)) => iApply refine_unit : core.
